Restructure `ASN1.*.Value.StringCombinator` (#47).

src/riot/asn1/ASN1.Low.Value.StringCombinator.fsti
@@ -20,10 +20,8 @@ module Cast = FStar.Int.Cast
 
 module B32 = FStar.Bytes
 
-friend ASN1.Spec.Value.StringCombinator
-
 noextract inline_for_extraction
-let serialize32_asn1_string_backwards
+val serialize32_asn1_string_backwards
   (t: asn1_type { t == IA5_STRING \/ t == PRINTABLE_STRING \/ t == OCTET_STRING })
   (len_of_string: datatype_of_asn1_type t -> asn1_value_int32_of_type t)
   (filter_string: (len: asn1_value_int32_of_type t)
@@ -40,24 +38,9 @@ let serialize32_asn1_string_backwards
   (prf: unit { forall len. synth_injective (synth_string len) })
   (len: asn1_value_int32_of_type t)
 : Tot (serializer32_backwards (serialize_asn1_string t len_of_string filter_string synth_string synth_string_inverse prf len))
-= fun (x: datatype_of_asn1_type t { v (len_of_string x) == v len })
-    (#rrel #rel: _)
-    (b: B.mbuffer byte rrel rel)
-    (pos: size_t)
--> (* Prf *) lemma_serialize_asn1_string_unfold t len_of_string filter_string synth_string synth_string_inverse prf len x;
 
-    store_bytes
-    (* src *) (synth_string_inverse len x)
-    (* from*) 0ul
-    (* to  *) len
-    (* dst *) b
-    (* pos *) (pos - len);
-
-(* return *) len
-
-#push-options "--z3rlimit 32 --fuel 2 --ifuel 2"
 noextract inline_for_extraction
-let serialize32_asn1_string_TLV_backwards
+val serialize32_asn1_string_TLV_backwards
   (t: asn1_type { t == IA5_STRING \/ t == PRINTABLE_STRING \/ t == OCTET_STRING })
   (len_of_string: datatype_of_asn1_type t -> asn1_value_int32_of_type t)
   (filter_string: (len: asn1_value_int32_of_type t)
@@ -73,22 +56,9 @@ let serialize32_asn1_string_TLV_backwards
                                  { x == synth_string len s32 }))
   (prf: unit { forall len. synth_injective (synth_string len) })
 : serializer32_backwards (serialize_asn1_string_TLV t len_of_string filter_string synth_string synth_string_inverse prf)
-= serialize32_tagged_union_backwards
-  (* lst*) (serialize32_asn1_tag_of_type_backwards t
-            `serialize32_nondep_then_backwards`
-            serialize32_asn1_length_of_type_backwards t)
-  (* tg *) (fun x -> parser_tag_of_asn1_string t len_of_string x)
-  (* ls *) (fun x -> (serialize32_synth_backwards
-                    (* ls *) (weak_kind_of_type t
-                              `serialize32_weaken_backwards`
-                              serialize32_asn1_string_backwards t len_of_string filter_string synth_string synth_string_inverse prf (snd x))
-                    (* f2 *) (synth_asn1_string_V t len_of_string x)
-                    (* g1 *) (synth_asn1_string_V_inverse t len_of_string x)
-                    (* g1'*) (synth_asn1_string_V_inverse t len_of_string x)
-                    (* prf*) ()))
 
 noextract inline_for_extraction
-let serialize32_asn1_string_TLV_with_character_bound_backwards
+val serialize32_asn1_string_TLV_with_character_bound_backwards
   (t: asn1_type { t == IA5_STRING \/ t == PRINTABLE_STRING \/ t == OCTET_STRING })
   (len_of_string: datatype_of_asn1_type t -> asn1_value_int32_of_type t)
   (filter_string: (len: asn1_value_int32_of_type t)
@@ -107,6 +77,3 @@ let serialize32_asn1_string_TLV_with_character_bound_backwards
   (lb: asn1_value_int32_of_type t)
   (ub: asn1_value_int32_of_type t { lb <= ub })
 : serializer32_backwards (serialize_asn1_string_TLV_with_character_bound t len_of_string filter_string synth_string synth_string_inverse prf count_character lb ub)
-= serialize32_asn1_string_TLV_backwards t len_of_string filter_string synth_string synth_string_inverse prf
-  `serialize32_filter_backwards`
-  filter_asn1_string_with_character_bound t count_character lb ub
