src/riot/asn1/ASN1.Spec.Value.StringCombinator.fsti
@@ -11,7 +11,12 @@ open FStar.Integers
 
 module B32 = FStar.Bytes
 
-let parse_asn1_string
+let parse_asn1_string_kind
+  (t: asn1_type { t == IA5_STRING \/ t == PRINTABLE_STRING \/ t == OCTET_STRING })
+  (len: asn1_value_int32_of_type t)
+= parse_filter_kind (total_constant_size_parser_kind (v len))
+
+val parse_asn1_string
   (t: asn1_type { t == IA5_STRING \/ t == PRINTABLE_STRING \/ t == OCTET_STRING })
   (len_of_string: datatype_of_asn1_type t -> asn1_value_int32_of_type t)
   (filter_string: (len: asn1_value_int32_of_type t)
@@ -23,14 +28,9 @@ let parse_asn1_string
                                   { len_of_string x== len }))
   (prf: unit { forall len. synth_injective (synth_string len) })
   (len: asn1_value_int32_of_type t)
-: parser _ (x: datatype_of_asn1_type t {len_of_string x == len})
-= parse_flbytes (v len)
-  `parse_filter`
-  filter_string len
-  `parse_synth`
-  synth_string len
+: parser (parse_asn1_string_kind t len) (x: datatype_of_asn1_type t {len_of_string x == len})
 
-let serialize_asn1_string
+val serialize_asn1_string
   (t: asn1_type { t == IA5_STRING \/ t == PRINTABLE_STRING \/ t == OCTET_STRING })
   (len_of_string: datatype_of_asn1_type t -> asn1_value_int32_of_type t)
   (filter_string: (len: asn1_value_int32_of_type t)
@@ -47,18 +47,29 @@ let serialize_asn1_string
   (prf: unit { forall len. synth_injective (synth_string len) })
   (len: asn1_value_int32_of_type t)
 : serializer (parse_asn1_string t len_of_string filter_string synth_string prf len)
-= serialize_synth
-  (* p1 *) (parse_flbytes (v len)
-            `parse_filter`
-            filter_string len)
-  (* f2 *) (synth_string len)
-  (* s1 *) (serialize_flbytes (v len)
-            `serialize_filter`
-            filter_string len)
-  (* g1 *) (synth_string_inverse len)
-  (* Prf*) (prf)
 
-let lemma_serialize_asn1_string_unfold
+let predicate_serialize_asn1_string_unfold
+  (t: asn1_type { t == IA5_STRING \/ t == PRINTABLE_STRING \/ t == OCTET_STRING })
+  (len_of_string: datatype_of_asn1_type t -> asn1_value_int32_of_type t)
+  (filter_string: (len: asn1_value_int32_of_type t)
+                  -> (s32: B32.lbytes32 len)
+                  -> GTot (bool))
+  (synth_string: (len: asn1_value_int32_of_type t)
+                 -> (s32: parse_filter_refine (filter_string len))
+                 -> GTot (x: datatype_of_asn1_type t
+                            { len_of_string x== len }))
+  (synth_string_inverse: (len: asn1_value_int32_of_type t)
+                         -> (x: datatype_of_asn1_type t { len_of_string x== len })
+                         -> (s32: parse_filter_refine (filter_string len)
+                                 { x == synth_string len s32 }))
+  (prf: unit { forall len. synth_injective (synth_string len) })
+  (len: asn1_value_int32_of_type t)
+  (x: datatype_of_asn1_type t { len_of_string x== len })
+: Type0
+= serialize (serialize_asn1_string t len_of_string filter_string synth_string synth_string_inverse prf len) x
+  == serialize (serialize_flbytes (v len)) (synth_string_inverse len x)
+
+val lemma_serialize_asn1_string_unfold
   (t: asn1_type { t == IA5_STRING \/ t == PRINTABLE_STRING \/ t == OCTET_STRING })
   (len_of_string: datatype_of_asn1_type t -> asn1_value_int32_of_type t)
   (filter_string: (len: asn1_value_int32_of_type t)
@@ -78,19 +89,31 @@ let lemma_serialize_asn1_string_unfold
 : Lemma (
   predicate_serialize_asn1_string_unfold t len_of_string filter_string synth_string synth_string_inverse prf len x
 )
-= serialize_synth_eq
-  (* p1 *) (parse_flbytes (v len)
-            `parse_filter`
-            filter_string len)
-  (* f2 *) (synth_string len)
-  (* s1 *) (serialize_flbytes (v len)
-            `serialize_filter`
-            filter_string len)
-  (* g1 *) (synth_string_inverse len)
-  (* Prf*) (prf)
-  (* in *) (x)
 
-let lemma_serialize_asn1_string_size
+let predicate_serialize_asn1_string_size
+  (t: asn1_type { t == IA5_STRING \/ t == PRINTABLE_STRING \/ t == OCTET_STRING })
+  (len_of_string: datatype_of_asn1_type t -> asn1_value_int32_of_type t)
+  (filter_string: (len: asn1_value_int32_of_type t)
+                  -> (s32: B32.lbytes32 len)
+                  -> GTot (bool))
+  (synth_string: (len: asn1_value_int32_of_type t)
+                 -> (s32: parse_filter_refine (filter_string len))
+                 -> GTot (x: datatype_of_asn1_type t
+                            { len_of_string x== len }))
+  (synth_string_inverse: (len: asn1_value_int32_of_type t)
+                         -> (x: datatype_of_asn1_type t { len_of_string x== len })
+                         -> (s32: parse_filter_refine (filter_string len)
+                                 { x == synth_string len s32 }))
+  (prf: unit { forall len. synth_injective (synth_string len) })
+  (len: asn1_value_int32_of_type t)
+  (x: datatype_of_asn1_type t { len_of_string x== len })
+: Type0
+= let length = length_of_opaque_serialization (serialize_asn1_string t len_of_string filter_string synth_string synth_string_inverse prf len) x in
+  length == v len /\
+  len == len_of_string x /\
+  asn1_value_length_inbound_of_type t length
+
+val lemma_serialize_asn1_string_size
   (t: asn1_type { t == IA5_STRING \/ t == PRINTABLE_STRING \/ t == OCTET_STRING })
   (len_of_string: datatype_of_asn1_type t -> asn1_value_int32_of_type t)
   (filter_string: (len: asn1_value_int32_of_type t)
@@ -110,116 +133,21 @@ let lemma_serialize_asn1_string_size
 : Lemma (
   predicate_serialize_asn1_string_size t len_of_string filter_string synth_string synth_string_inverse prf len x
 )
-= lemma_serialize_asn1_string_unfold t len_of_string filter_string synth_string synth_string_inverse prf len x
 
-noextract inline_for_extraction
-let parser_tag_of_asn1_string
+
+
+
+
+let parse_asn1_string_TLV_kind
   (t: asn1_type { t == IA5_STRING \/ t == PRINTABLE_STRING \/ t == OCTET_STRING })
-  (len_of_string: datatype_of_asn1_type t -> asn1_value_int32_of_type t)
-  (x: datatype_of_asn1_type t)
-: Tot (the_asn1_tag t `tuple2` asn1_value_int32_of_type t)
-= (t, len_of_string x)
+: parser_kind
+= parse_asn1_tag_kind
+  `and_then_kind`
+  parse_asn1_length_kind_of_type t
+  `and_then_kind`
+  weak_kind_of_type t
 
-let synth_asn1_string_V
-  (t: asn1_type { t == IA5_STRING \/ t == PRINTABLE_STRING \/ t == OCTET_STRING })
-  (len_of_string: datatype_of_asn1_type t -> asn1_value_int32_of_type t)
-  (tag: the_asn1_tag t `tuple2` asn1_value_int32_of_type t)
-  (value: datatype_of_asn1_type t { v (len_of_string value) == v (snd tag) })
-: GTot (refine_with_tag (parser_tag_of_asn1_string t len_of_string) tag)
-= value
-
-noextract inline_for_extraction
-let synth_asn1_string_V_inverse
-  (t: asn1_type { t == IA5_STRING \/ t == PRINTABLE_STRING \/ t == OCTET_STRING })
-  (len_of_string: datatype_of_asn1_type t -> asn1_value_int32_of_type t)
-  (tag: the_asn1_tag t `tuple2` asn1_value_int32_of_type t)
-  (value': refine_with_tag (parser_tag_of_asn1_string t len_of_string) tag)
-: Tot (value: datatype_of_asn1_type t
-               { v (len_of_string value) == v (snd tag) /\
-                 value' == synth_asn1_string_V t len_of_string tag value })
-= value'
-
-let parse_asn1_string_V
-  (t: asn1_type { t == IA5_STRING \/ t == PRINTABLE_STRING \/ t == OCTET_STRING })
-  (len_of_string: datatype_of_asn1_type t -> asn1_value_int32_of_type t)
-  (filter_string: (len: asn1_value_int32_of_type t)
-                  -> (s32: B32.lbytes32 len)
-                  -> GTot (bool))
-  (synth_string: (len: asn1_value_int32_of_type t)
-                       -> (s32: parse_filter_refine (filter_string len))
-                       -> GTot (x: datatype_of_asn1_type t
-                                  { len_of_string x== len }))
-  (prf: unit { forall len. synth_injective (synth_string len) })
-  (tag: the_asn1_tag t `tuple2` asn1_value_int32_of_type t)
-: parser (weak_kind_of_type t) (refine_with_tag (parser_tag_of_asn1_string t len_of_string) tag)
-= weak_kind_of_type t
-  `weaken`
-  parse_asn1_string t len_of_string filter_string synth_string prf (snd tag)
-  `parse_synth`
-  synth_asn1_string_V t len_of_string tag
-
-let serialize_asn1_string_V
-  (t: asn1_type { t == IA5_STRING \/ t == PRINTABLE_STRING \/ t == OCTET_STRING })
-  (len_of_string: datatype_of_asn1_type t -> asn1_value_int32_of_type t)
-  (filter_string: (len: asn1_value_int32_of_type t)
-                  -> (s32: B32.lbytes32 len)
-                  -> GTot (bool))
-  (synth_string: (len: asn1_value_int32_of_type t)
-                 -> (s32: parse_filter_refine (filter_string len))
-                 -> GTot (x: datatype_of_asn1_type t
-                            { len_of_string x== len }))
-  (synth_string_inverse: (len: asn1_value_int32_of_type t)
-                         -> (x: datatype_of_asn1_type t { len_of_string x== len })
-                         -> (s32: parse_filter_refine (filter_string len)
-                                 { x == synth_string len s32 }))
-  (prf: unit { forall len. synth_injective (synth_string len) })
-  (tag: the_asn1_tag t `tuple2` asn1_value_int32_of_type t)
-: serializer (parse_asn1_string_V t len_of_string filter_string synth_string prf tag)
-= serialize_synth
-  (* p1 *) (weak_kind_of_type t
-            `weaken`
-            parse_asn1_string t len_of_string filter_string synth_string prf (snd tag))
-  (* f2 *) (synth_asn1_string_V t len_of_string tag)
-  (* s1 *) (weak_kind_of_type t
-            `serialize_weaken`
-            serialize_asn1_string t len_of_string filter_string synth_string synth_string_inverse prf (snd tag))
-  (* g1 *) (synth_asn1_string_V_inverse t len_of_string tag)
-  (* prf*) (prf)
-
-let lemma_serialize_asn1_string_V_unfold
-  (t: asn1_type { t == IA5_STRING \/ t == PRINTABLE_STRING \/ t == OCTET_STRING })
-  (len_of_string: datatype_of_asn1_type t -> asn1_value_int32_of_type t)
-  (filter_string: (len: asn1_value_int32_of_type t)
-                  -> (s32: B32.lbytes32 len)
-                  -> GTot (bool))
-  (synth_string: (len: asn1_value_int32_of_type t)
-                 -> (s32: parse_filter_refine (filter_string len))
-                 -> GTot (x: datatype_of_asn1_type t
-                            { len_of_string x== len }))
-  (synth_string_inverse: (len: asn1_value_int32_of_type t)
-                         -> (x: datatype_of_asn1_type t { len_of_string x== len })
-                         -> (s32: parse_filter_refine (filter_string len)
-                                 { x == synth_string len s32 }))
-  (prf: unit { forall len. synth_injective (synth_string len) })
-  (tag: the_asn1_tag t `tuple2` asn1_value_int32_of_type t)
-  (x: refine_with_tag (parser_tag_of_asn1_string t len_of_string) tag)
-: Lemma (
-  serialize (serialize_asn1_string_V t len_of_string filter_string synth_string synth_string_inverse prf tag) x ==
-  serialize (serialize_asn1_string t len_of_string filter_string synth_string synth_string_inverse prf (snd tag)) x
-)
-= serialize_synth_eq
-  (* p1 *) (weak_kind_of_type t
-            `weaken`
-            parse_asn1_string t len_of_string filter_string synth_string prf (snd tag))
-  (* f2 *) (synth_asn1_string_V t len_of_string tag)
-  (* s1 *) (weak_kind_of_type t
-            `serialize_weaken`
-            serialize_asn1_string t len_of_string filter_string synth_string synth_string_inverse prf (snd tag))
-  (* g1 *) (synth_asn1_string_V_inverse t len_of_string tag)
-  (* prf*) (prf)
-  (* in *) (x)
-
-let parse_asn1_string_TLV
+val parse_asn1_string_TLV
   (t: asn1_type { t == IA5_STRING \/ t == PRINTABLE_STRING \/ t == OCTET_STRING })
   (len_of_string: datatype_of_asn1_type t -> asn1_value_int32_of_type t)
   (filter_string: (len: asn1_value_int32_of_type t)
@@ -231,14 +159,8 @@ let parse_asn1_string_TLV
                                   { len_of_string x== len }))
   (prf: unit { forall len. synth_injective (synth_string len) })
 : parser (parse_asn1_string_TLV_kind t) (datatype_of_asn1_type t)
-= parse_tagged_union
-  (* pt *) (parse_asn1_tag_of_type t
-            `nondep_then`
-            parse_asn1_length_of_type t)
-  (* tg *) (parser_tag_of_asn1_string t len_of_string)
-  (* p  *) (parse_asn1_string_V t len_of_string filter_string synth_string prf)
 
-let serialize_asn1_string_TLV
+val serialize_asn1_string_TLV
   (t: asn1_type { t == IA5_STRING \/ t == PRINTABLE_STRING \/ t == OCTET_STRING })
   (len_of_string: datatype_of_asn1_type t -> asn1_value_int32_of_type t)
   (filter_string: (len: asn1_value_int32_of_type t)
@@ -254,15 +176,32 @@ let serialize_asn1_string_TLV
                                  { x == synth_string len s32 }))
   (prf: unit { forall len. synth_injective (synth_string len) })
 : serializer (parse_asn1_string_TLV t len_of_string filter_string synth_string prf)
-= serialize_tagged_union
-  (* st *) (serialize_asn1_tag_of_type t
-            `serialize_nondep_then`
-            serialize_asn1_length_of_type t)
-  (* tg *) (parser_tag_of_asn1_string t len_of_string)
-  (* s  *) (serialize_asn1_string_V t len_of_string filter_string synth_string synth_string_inverse prf)
 
-#push-options "--z3rlimit 32"
-let lemma_serialize_asn1_string_TLV_unfold
+let predicate_serialize_asn1_string_TLV_unfold
+  (t: asn1_type { t == IA5_STRING \/ t == PRINTABLE_STRING \/ t == OCTET_STRING })
+  (len_of_string: datatype_of_asn1_type t -> asn1_value_int32_of_type t)
+  (filter_string: (len: asn1_value_int32_of_type t)
+                  -> (s32: B32.lbytes32 len)
+                  -> GTot (bool))
+  (synth_string: (len: asn1_value_int32_of_type t)
+                       -> (s32: parse_filter_refine (filter_string len))
+                       -> GTot (x: datatype_of_asn1_type t
+                                  { len_of_string x== len }))
+  (synth_string_inverse: (len: asn1_value_int32_of_type t)
+                         -> (x: datatype_of_asn1_type t { len_of_string x== len })
+                         -> (s32: parse_filter_refine (filter_string len)
+                                 { x == synth_string len s32 }))
+  (prf: unit { forall len. synth_injective (synth_string len) })
+  (x: datatype_of_asn1_type t)
+: Type0
+= serialize (serialize_asn1_string_TLV t len_of_string filter_string synth_string synth_string_inverse prf) x ==
+  serialize (serialize_asn1_tag_of_type t) t
+  `Seq.append`
+  serialize (serialize_asn1_length_of_type t) (len_of_string x)
+  `Seq.append`
+  serialize (serialize_asn1_string t len_of_string filter_string synth_string synth_string_inverse prf (len_of_string x)) x
+
+val lemma_serialize_asn1_string_TLV_unfold
   (t: asn1_type { t == IA5_STRING \/ t == PRINTABLE_STRING \/ t == OCTET_STRING })
   (len_of_string: datatype_of_asn1_type t -> asn1_value_int32_of_type t)
   (filter_string: (len: asn1_value_int32_of_type t)
@@ -281,20 +220,29 @@ let lemma_serialize_asn1_string_TLV_unfold
 : Lemma (
   predicate_serialize_asn1_string_TLV_unfold t len_of_string filter_string synth_string synth_string_inverse prf x
 )
-= serialize_nondep_then_eq
-  (* s1 *) (serialize_asn1_tag_of_type t)
-  (* s2 *) (serialize_asn1_length_of_type t)
-  (* in *) (parser_tag_of_asn1_string t len_of_string x);
-  lemma_serialize_asn1_string_V_unfold t len_of_string filter_string synth_string synth_string_inverse prf (parser_tag_of_asn1_string t len_of_string x) x;
-  serialize_tagged_union_eq
-  (* st *) (serialize_asn1_tag_of_type t
-            `serialize_nondep_then`
-            serialize_asn1_length_of_type t)
-  (* tg *) (parser_tag_of_asn1_string t len_of_string)
-  (* s  *) (serialize_asn1_string_V t len_of_string filter_string synth_string synth_string_inverse prf)
-  (* in *) (x)
 
-let lemma_serialize_asn1_string_TLV_size
+let predicate_serialize_asn1_string_TLV_size
+  (t: asn1_type { t == IA5_STRING \/ t == PRINTABLE_STRING \/ t == OCTET_STRING })
+  (len_of_string: datatype_of_asn1_type t -> asn1_value_int32_of_type t)
+  (filter_string: (len: asn1_value_int32_of_type t)
+                  -> (s32: B32.lbytes32 len)
+                  -> GTot (bool))
+  (synth_string: (len: asn1_value_int32_of_type t)
+                       -> (s32: parse_filter_refine (filter_string len))
+                       -> GTot (x: datatype_of_asn1_type t
+                                  { len_of_string x== len }))
+  (synth_string_inverse: (len: asn1_value_int32_of_type t)
+                         -> (x: datatype_of_asn1_type t { len_of_string x== len })
+                         -> (s32: parse_filter_refine (filter_string len)
+                                 { x == synth_string len s32 }))
+  (prf: unit { forall len. synth_injective (synth_string len) })
+  (x: datatype_of_asn1_type t)
+: Type0
+= let length: nat = length_of_opaque_serialization (serialize_asn1_string_TLV t len_of_string filter_string synth_string synth_string_inverse prf) x in
+  length == 1 + length_of_asn1_length (len_of_string x) + v (len_of_string x) /\
+  asn1_TLV_length_inbound_of_type t length
+
+val lemma_serialize_asn1_string_TLV_size
   (t: asn1_type { t == IA5_STRING \/ t == PRINTABLE_STRING \/ t == OCTET_STRING })
   (len_of_string: datatype_of_asn1_type t -> asn1_value_int32_of_type t)
   (filter_string: (len: asn1_value_int32_of_type t)
@@ -313,16 +261,27 @@ let lemma_serialize_asn1_string_TLV_size
 : Lemma (
   predicate_serialize_asn1_string_TLV_size t len_of_string filter_string synth_string synth_string_inverse prf x
 )
-= lemma_serialize_asn1_string_TLV_unfold t len_of_string filter_string synth_string synth_string_inverse prf x;
-  lemma_serialize_asn1_tag_of_type_size t t;
-  lemma_serialize_asn1_length_size (len_of_string x);
-  serialize_asn1_length_of_type_eq t (len_of_string x);
-  lemma_serialize_asn1_string_size t len_of_string filter_string synth_string synth_string_inverse prf (len_of_string x) x
-#pop-options
 
 
 
-let parse_asn1_string_TLV_with_character_bound
+let filter_asn1_string_with_character_bound
+  (t: asn1_type { t == IA5_STRING \/ t == PRINTABLE_STRING \/ t == OCTET_STRING })
+  (count_character: (x: datatype_of_asn1_type t) -> Tot (asn1_int32))
+  (lb: asn1_value_int32_of_type t)
+  (ub: asn1_value_int32_of_type t { lb <= ub })
+  (x: datatype_of_asn1_type t)
+: Tot (bool)
+= lb <= count_character x && count_character x <= ub
+
+noextract inline_for_extraction
+let asn1_string_with_character_bound_t
+  (t: asn1_type { t == IA5_STRING \/ t == PRINTABLE_STRING \/ t == OCTET_STRING })
+  (count_character: (x: datatype_of_asn1_type t) -> Tot (asn1_int32))
+  (lb: asn1_value_int32_of_type t)
+  (ub: asn1_value_int32_of_type t { lb <= ub })
+= parse_filter_refine (filter_asn1_string_with_character_bound t count_character lb ub)
+
+val parse_asn1_string_TLV_with_character_bound
   (t: asn1_type { t == IA5_STRING \/ t == PRINTABLE_STRING \/ t == OCTET_STRING })
   (len_of_string: datatype_of_asn1_type t -> asn1_value_int32_of_type t)
   (filter_string: (len: asn1_value_int32_of_type t)
@@ -337,11 +296,8 @@ let parse_asn1_string_TLV_with_character_bound
   (lb: asn1_value_int32_of_type t)
   (ub: asn1_value_int32_of_type t { lb <= ub })
 : parser (parse_asn1_string_TLV_kind t) (asn1_string_with_character_bound_t t count_character lb ub)
-= parse_asn1_string_TLV t len_of_string filter_string synth_string prf
-  `parse_filter`
-  filter_asn1_string_with_character_bound t count_character lb ub
 
-let serialize_asn1_string_TLV_with_character_bound
+val serialize_asn1_string_TLV_with_character_bound
   (t: asn1_type { t == IA5_STRING \/ t == PRINTABLE_STRING \/ t == OCTET_STRING })
   (len_of_string: datatype_of_asn1_type t -> asn1_value_int32_of_type t)
   (filter_string: (len: asn1_value_int32_of_type t)
@@ -360,6 +316,3 @@ let serialize_asn1_string_TLV_with_character_bound
   (lb: asn1_value_int32_of_type t)
   (ub: asn1_value_int32_of_type t { lb <= ub })
 : serializer (parse_asn1_string_TLV_with_character_bound t len_of_string filter_string synth_string prf count_character lb ub)
-= serialize_asn1_string_TLV t len_of_string filter_string synth_string synth_string_inverse prf
-  `serialize_filter`
-  filter_asn1_string_with_character_bound t count_character lb ub
